aneris/examples/snapshot_isolation/proof/model.v
@@ -76,6 +76,8 @@ End Whist_valid.
     for both, which gives a very simple kvs model coherence. In particular, if the global time is strictly
     positive, it does not imply that any commit happened previously. *)
 
+(** Update: we do need to track start times separately. *)
+
 Section KVS_valid.
   Context `{!User_params}.
 
@@ -90,17 +92,40 @@ Section KVS_valid.
   Definition kvs_whist_commit_times (M : kvsMdl) (T : nat) :=
     ∀ k h, M !! k = Some h → ∀ e, e ∈ h → e.(we_time) <= T.
 
+  Definition time_tss_valid (T : nat) (Tss : gset nat) : Prop :=
+    ∀ (t : nat), t ∈ Tss → t ≤ T.
 
-  Record kvs_valid (M : kvsMdl) (T : nat) : Prop :=
+  Definition hist_cut_by_snap (h hl hr : list write_event) (t : nat) : Prop :=
+      h = hl ++ hr ∧
+      (∀ e, e ∈ hl → e.(we_time) < t) ∧
+      (∀ e, e ∈ hr → t < e.(we_time)).
+
+  (** There are several lemmas that we will probably need about valid cuts. *)
+
+  Lemma hist_cut_by_snap_unicity (h hl1 hr1 hl2 hr2 : list write_event) (t : nat) :
+    whist_ext h →
+    whist_times h →
+    hist_cut_by_snap h hl1 hr1 t →
+    hist_cut_by_snap h hl2 hr2 t →
+    hl1 = hl2 ∧ hr1 = hr2.
+  Proof.
+  Admitted.
+
+  Definition kvs_tss_valid (M : kvsMdl) (Tss : gset nat) : Prop :=
+    ∀ k h t, M !! k = Some h → t ∈ Tss → ∃ hl hr, hist_cut_by_snap h hl hr t.
+
+  Record kvs_valid (M : kvsMdl) (T : nat) (Tss : gset nat) : Prop :=
     {
       kvs_ValidDom: kvs_dom M;
       kvs_ValidWhists : kvs_whists M;
       kvs_ValidKeys : kvs_keys M;
       kvs_ValidCommitTimes : kvs_whist_commit_times M T;
+      kvs_ValidSnapshotTimesTime : time_tss_valid T Tss;
+      kvs_ValidSnapshotTimesCuts : kvs_tss_valid M Tss
     }.
 
   Lemma valid_state_empty :
-    kvs_valid (gset_to_gmap [] KVS_keys) 0.
+    kvs_valid (gset_to_gmap [] KVS_keys) 0 ∅.
   Proof.
     split; rewrite /kvs_ValidDom /kvs_dom /kvs_whists /kvs_ValidWhists /kvs_ValidCommitTimes.
     -  by rewrite dom_gset_to_gmap.
@@ -110,6 +135,8 @@ Section KVS_valid.
       apply lookup_gset_to_gmap_Some in Habs as [_ <-]. set_solver.
     - rewrite /kvs_whist_commit_times. intros ? ? Habs.
       apply lookup_gset_to_gmap_Some in Habs as [_ <-]. set_solver.
+    - by rewrite /time_tss_valid.
+    - by rewrite /kvs_tss_valid.
    Qed.
 
   Definition update_kvs (M0 : kvsMdl) (C : gmap Key SerializableVal) (T : nat) :=
@@ -120,26 +147,30 @@ Section KVS_valid.
              ]> M))
         M0 C.
 
-  Lemma kvs_valid_update_cell  (M : kvsMdl) (T : nat) (k : Key) (v : SerializableVal) :
+  (** Probably not needed as lemma! *)
+  Lemma kvs_valid_update_cell
+        (M : kvsMdl) (T : nat) (Tss : gset nat) (k : Key) (v : SerializableVal) :
     k ∈ KVS_keys →
-    kvs_valid M T ->
+    kvs_valid M T Tss ->
     kvs_valid
       (<[ k := (default [] (M !! k)) ++
                [{| we_key := k; we_val := v; we_time := (T + 1)%nat |}]
         ]> M)
-      (T+1).
+      (T+1) (Tss ∪ {[(T+1)%nat]}).
   Proof.
   Admitted.
 
-  Lemma kvs_valid_update  (M : kvsMdl) (T : nat) (cache : gmap Key SerializableVal) :
+  Lemma kvs_valid_update  (M : kvsMdl) (T : nat) (Tss : gset nat) (cache : gmap Key SerializableVal) :
     dom cache ⊆ KVS_keys →
-    kvs_valid M T ->
-    kvs_valid (update_kvs M cache (T+1)) (T+1).
+    kvs_valid M T Tss ->
+    kvs_valid (update_kvs M cache (T+1)) (T+1) (Tss ∪ {[(T+1)%nat]}).
   Proof.
   Admitted.
 
 
-Lemma kvs_valid_next M T : (kvs_valid M (T + 1)).
+Lemma kvs_valid_next M T Tss :
+  kvs_valid M T Tss →
+  kvs_valid M (T + 1) (Tss ∪ {[(T+1)%nat]}).
 Proof. Admitted.
 
 End KVS_valid.
@@ -161,17 +192,17 @@ Section KVSL_valid.
   Definition kvsl_in_local_some_coh (m : gmap Key val) (M : kvsMdl) :=
     ∀ k (h: whist), m !! k = Some $h → M !! k = Some (reverse h).
 
-  Record kvsl_valid (m : gmap Key val) (M : kvsMdl) (T : nat) : Prop :=
+  Record kvsl_valid (m : gmap Key val) (M : kvsMdl) (T : nat) (Tss : gset nat) : Prop :=
     {
       kvsl_ValidDom: kvsl_dom m;
       kvsl_ValidInModelEmpty : kvsl_in_model_empty_coh m M;
       kvsl_ValidInModelSome : kvsl_in_model_some_coh m M;
       kvsl_ValidLocalSome : kvsl_in_local_some_coh m M;
-      kvsl_ValidModel : kvs_valid M T
+      kvsl_ValidModel : kvs_valid M T Tss
     }.
 
   Lemma kvsl_valid_empty :
-    kvsl_valid ∅ (gset_to_gmap [] KVS_keys) 0.
+    kvsl_valid ∅ (gset_to_gmap [] KVS_keys) 0 ∅.
   Proof.
   Admitted.
 
@@ -182,15 +213,6 @@ Section KVSL_valid.
 (*            (<[ k := {| we_key := k; we_val := v.(SV_val); we_time := T |} :: default [] (M !! k)]> M)) *)
 (*         M0 C. *)
 
-(*   Lemma kvs_valid_update_cell  (M : kvsMdl) (T : nat) (k : Key) (v : SerializableVal) : *)
-(*     k ∈ KVS_keys → *)
-(*     kvs_valid M T -> *)
-(*     kvs_valid *)
-(*       (<[ k := {| we_key := k; we_val := v; we_time := (T + 1)%nat |} :: default [] (M !! k)]> M) *)
-(*       (T+1). *)
-(*   Proof. *)
-(*   Admitted. *)
-
 (*   Lemma kvs_valid_update  (M : kvsMdl) (T : nat) (cache : gmap Key SerializableVal) : *)
 (*     dom cache = KVS_keys → *)
 (*     kvs_valid M T -> *)
@@ -199,22 +221,30 @@ Section KVSL_valid.
 (*   Admitted. *)
 (* End KVSL_valid. *)
 
-Lemma kvsl_valid_next M (m : gmap Key val) T : kvsl_valid m M (T + 1).
+Lemma kvsl_valid_next M (m : gmap Key val) T Tss :
+  kvsl_valid m M T Tss →
+  kvsl_valid m M (T + 1) (Tss ∪ {[(T+1)%nat]}).
 Proof. Admitted.
+
+  Lemma kvs_valid_filter M (mu : gmap Key (list val)) T Tss :
+    kvs_valid M T Tss →
+    kvs_valid
+       (filter (λ k : Key * list write_event, k.1 ∈ dom mu) M)
+       T Tss.
+  Proof.
+  Admitted.
 
 End KVSL_valid.
 
 Section Snapshot.
   Context `{!User_params}.
 
-  Definition kvs_valid_snapshot (M : gmap Key (list write_event)) (t : Time) :=
-   kvs_valid M t ∧
+  Definition kvs_valid_snapshot
+             (M : gmap Key (list write_event)) (t : Time) (Tss : gset nat)  :=
+   t ∈ Tss ∧
+   kvs_valid M t Tss ∧
    ∀ k h, M !! k = Some h → ∀ e, e ∈ h → e.(we_time) < t.
 
-  Lemma kvs_valid_snapshot_filter_next M (mu : gmap Key (list val)) T :
-    (kvs_valid_snapshot
-       (filter (λ k : Key * list write_event, k.1 ∈ dom mu) M)
-       (T + 1)%nat).
-  Proof. Admitted.
+
 
 End Snapshot.
