aneris/examples/snapshot_isolation/proof/server/proof_of_read_handler.v
@@ -31,25 +31,34 @@ Section Proof_of_read_handler.
 
   Context `{!anerisG Mdl Σ, !User_params, !IDBG Σ}.
   Context (clients : gset socket_address).
-  Context (γKnownClients γGauth γGsnap γT γlk : gname).
+  Context (γKnownClients γGauth γGsnap γT γTss γlk : gname).
   Context (srv_si : message → iProp Σ).
   Notation MTC := (client_handler_rpc_user_params
-                     clients γKnownClients γGauth γGsnap γT).
+                     clients γKnownClients γGauth γGsnap γT γTss).
   Import snapshot_isolation_code_api.
   Import assert_proof.
 
-  Lemma kvs_get_spec (k : Key) (kvsV : val) (h : list write_event)
+  Lemma kvs_get_spec (k : Key) (kvsV : val)
+        (Hh : list write_event)
        (m : gmap Key val) (M : gmap Key (list write_event)) :
    is_map kvsV m →
-   M !! k = Some h →
+   M !! k = Some Hh →
    kvsl_in_model_empty_coh m M →
    kvsl_in_model_some_coh m M →
    kvsl_in_local_some_coh m M →
    {{{ ⌜True⌝ }}}
        kvs_get #k kvsV  @[ip_of_address MTC.(MTS_saddr)]
-    {{{ v, RET v; ⌜v = $(reverse h)⌝ ∧
-                 ((⌜v = InjLV #()⌝ ∗ ⌜h = []⌝) ∨
-                  (∃ e h', ⌜v = InjRV ($e, $h')⌝ ∗ ⌜h = (reverse (e :: h'))⌝))
+    {{{ (vlo : option (list write_event)) (v : val), RET v;
+        ⌜match vlo with
+         | None =>
+             v = NONEV ∧
+             Hh = []
+         | Some l =>
+             v = $l ∧
+             m !! k = Some v ∧
+             l ≠ [] ∧
+             l = reverse Hh
+         end⌝
     }}}.
   Proof.
     iIntros (Hmap HMk Hc1 Hc2 Hc3 Φ) "_ HΦ".
@@ -57,13 +66,13 @@ Section Proof_of_read_handler.
     wp_pures.
     wp_apply (wp_map_lookup $! Hmap).
     iIntros (v) "%Hkv".
-    destruct h as [|e h'] eqn:Hh; simplify_eq /=.
+    destruct Hh as [|e h'] eqn:Heq; simplify_eq /=.
     - specialize (Hc1 k HMk).
       destruct (m !! k) as [hv | ] eqn:Hmk; first done.
       simplify_eq /=.
       do 3 wp_pure _.
       wp_pures.
-      by iApply ("HΦ"); eauto.
+      by iApply ("HΦ" $! None).
     - destruct (m !! k) as [hv | ] eqn:Hmk.
       2: { specialize (Hc2 k (e :: h') HMk).
            naive_solver. }
@@ -81,28 +90,20 @@ Section Proof_of_read_handler.
          iSplit; first done.
          iNext.
          wp_pures.
-         iApply "HΦ".
-         iSplit; first done.
-         iRight.
-         iExists _, _.
-         iPureIntro.
-         split; first done.
-         apply Inj_instance_2.
-         rewrite Hrev.
-         by rewrite reverse_involutive.
+         by iApply ("HΦ" $! (Some (x :: l))).
   Qed.
 
-  Lemma kvs_get_last_spec (k : Key) (ts : nat) (T : nat) (kvsV : val)
+  Lemma kvs_get_last_spec (k : Key) (ts : nat) (T : nat) (Tss : gset nat) (kvsV : val)
         (h Hk : list write_event)
        (m : gmap Key val) (M : gmap Key (list write_event)) :
    (∀ e : events.write_event, e ∈ h → we_time e < ts) →
    is_map kvsV m →
-   kvsl_valid m M T →
+   kvsl_valid m M T Tss →
    ts < T →
    M !! k = Some Hk →
    h `prefix_of` Hk →
     {{{
-          ownTimeSnap γT ts ∗
+          ownTimeSnap γT γTss ts ∗
           ownMemSeen γGsnap k h ∗
           ownMemSeen γGsnap k Hk
     }}}
@@ -110,48 +111,157 @@ Section Proof_of_read_handler.
     {{{ (vo : option val), RET $vo;
         (⌜$vo = InjLV #()⌝ ∗ ⌜h = []⌝ ∨
         (∃ e : events.write_event, ⌜$vo = InjRV (we_val e)⌝ ∗
-             ⌜hist_to_we (reverse h) = Some e⌝))
+             ⌜hist_to_we h = Some e⌝))
     }}}.
   Proof.
     iIntros (Het Hm Hcoh HtT Hin Hpre Φ) "(#Ht & #Hsh & #HsH) HΦ".
     wp_lam.
-    wp_pures.
+    do 15 wp_pures.
     destruct Hcoh.
-    wp_smart_apply (kvs_get_spec k kvsV Hk m M Hm Hin ); eauto.
-    iIntros (vget Hget).
-    destruct Hget as (Hget & [(<- & ->) | (hv &  Hhv & Heq1 & Heq2)]).
-    - apply prefix_nil_inv in Hpre.
-      rewrite Hget.
-      rewrite reverse_nil.
+    wp_smart_apply (kvs_get_spec k kvsV Hk m M Hm Hin); eauto.
+    iIntros (vlo v) "%Hvlo".
+    iLöb as "IH" forall (v Hk vlo Hin Hpre Hvlo) "HsH".
+    destruct vlo as [l | ] eqn: Hvloeq; last first.
+    - destruct Hvlo as (-> & ->).
+      apply prefix_nil_inv in Hpre.
+      subst.
       wp_pures.
       iApply ("HΦ" $! None); eauto.
-    - rewrite Heq1.
-      iLöb as "IH".
+    - destruct Hvlo as (Hvl & Hmk & Hlneq & HlHk).
+      rewrite Hvl HlHk.
+      assert (∃ e Hr, reverse Hk = e :: (reverse Hr)) as (e & Hr & HkLast).
+      { admit. }
+      rewrite HkLast.
       wp_pures.
       case_bool_decide.
-      (** should be proven by contradiction. *)
+      (** should be proven by contradiction: *)
+(*            we_time hv.t = ts *)
+(*            either hv ∈ h, then hv.t < ts *)
+(*            or hv ∉ h but hv ∈ Hk, then ts < hv.t *)
       { admit. }
       wp_pures.
       case_bool_decide.
       { wp_pures.
-        iApply ("HΦ" $! (Some (we_val hv))).
+        iApply ("HΦ" $! (Some (we_val e))).
         iRight.
+        iExists e.
+        iSplit; first done.
         iPureIntro.
-        exists hv.
-        split; first done.
-        assert (Some hv = last (reverse (hv :: Hhv))) as HvkL.
-        { assert (Some hv = head (hv :: Hhv)) as ->. done.
-          by rewrite last_reverse. }
-        rewrite /hist_to_we.
-        rewrite HvkL.
-        assert ((reverse h) `suffix_of` (reverse (hv :: Hhv))) as Hsuf.
-        { rewrite Heq2 in Hpre.
-          admit. }
-        admit.
-      }
+        admit. }
       wp_pure _.
-      (* iApply ("IH" with "[$HΦ]"). *)
-   Admitted.
+      iApply ("IH" $! ($(reverse Hr)) Hr with "[][][][$HΦ]").
+      + admit.
+      + admit.
+      + admit.
+      + admit.
+  Admitted.
+    (*   iPureIntro. *)
+ (*      split. *)
+ (*      -- simpl.  *)
+ (*      split_and!; eauto. done. *)
+ (*    (** --------------------------- old stuff --------------------------- *) *)
+ (*    destruct Hget as (Hget & Hdis). *)
+ (*    rewrite Hget. *)
+
+ (*    iLöb as "IH". *)
+ (*    destruct Hdis as [(Hvgeteq & Hkeq) | (hv &  Hhv & Heq1 & Heq2)]. *)
+
+ (*    - rewrite -Hget Heq1.   *)
+ (*      wp_pures. *)
+ (*      case_bool_decide. *)
+ (*      (** should be proven by contradiction:  *) *)
+(*  (*           we_time hv.t = ts  *) *)
+(*  (*           either hv ∈ h, then hv.t < ts *) *)
+(*  (*           or hv ∉ h but hv ∈ Hk, then ts < hv.t *) *)
+ (*      { admit. } *)
+ (*      wp_pures. *)
+ (*      case_bool_decide. *)
+ (*      { wp_pures.  *)
+ (*        iApply ("HΦ" $! (Some (we_val hv))). *)
+ (*        iRight. *)
+ (*        iExists hv. *)
+ (*        iSplit; first done. *)
+ (*        iPureIntro. *)
+ (*        admit. } *)
+ (*      wp_pure _.  *)
+
+ (*    (* --------------------------------------------------------------------- *) *)
+ (*    iLöb as "IH"forall (Hk Hget Hin Hpre Hdis) "HsH". *)
+ (*    destruct Hdis as [(Hvgeteq & Hkeq) | (hv &  Hhv & Heq1 & Heq2)]. *)
+ (*    - subst.  *)
+ (*      apply prefix_nil_inv in Hpre. *)
+ (*      rewrite reverse_nil. *)
+ (*      wp_pures. *)
+ (*      iApply ("HΦ" $! None); eauto. *)
+ (*    - rewrite -Hget Heq1.   *)
+ (*      wp_pures. *)
+ (*      case_bool_decide. *)
+ (*      (** should be proven by contradiction:  *) *)
+(*  (*           we_time hv.t = ts  *) *)
+(*  (*           either hv ∈ h, then hv.t < ts *) *)
+(*  (*           or hv ∉ h but hv ∈ Hk, then ts < hv.t *) *)
+ (*      { admit. } *)
+ (*      wp_pures. *)
+ (*      case_bool_decide. *)
+ (*      { wp_pures.  *)
+ (*        iApply ("HΦ" $! (Some (we_val hv))). *)
+ (*        iRight. *)
+ (*        iExists hv. *)
+ (*        iSplit; first done. *)
+ (*        iPureIntro. *)
+ (*        admit. } *)
+ (*      wp_pure _.  *)
+
+ (*      assert ($ Hhv = reverse  *)
+ (*      iDestruct ("IH" $! . *)
+ (* destruct (reverse Hk) as [| e Hkl] eqn: Hkeq; first done. *)
+ (*      wp_pures. *)
+ (*      case_bool_decide. *)
+ (*      (** should be proven by contradiction. *) *)
+ (*      { admit. } *)
+ (*      wp_pures. *)
+ (*      case_bool_decide. *)
+ (*      { wp_pures. *)
+ (*        iApply ("HΦ" $! (Some (we_val e))). *)
+ (*         iRight. *)
+ (*         iExists e. *)
+ (*         iSplit; first done. *)
+ (*         iPureIntro. *)
+ (*      -- apply prefix_nil_inv in Hpre. *)
+ (*         rewrite reverse_nil. *)
+ (*         wp_pures. *)
+ (*         iApply ("HΦ" $! None); eauto. *)
+ (*      --        list_simplifier. *)
+ (*         simpl in Heq1. *)
+ (*         inversion Heq1. *)
+ (*         rewrite Heq2. *)
+ (*         rewrite reverse_involutive. *)
+ (*         wp_pures. *)
+ (*      case_bool_decide. *)
+ (*      (** should be proven by contradiction. *) *)
+ (*      { admit. } *)
+ (*      wp_pures. *)
+ (*      case_bool_decide. *)
+ (*      { wp_pures. *)
+ (*        iApply ("HΦ" $! (Some (we_val hv))). *)
+ (*        iRight. *)
+ (*        iPureIntro. *)
+ (*        exists hv. *)
+ (*        split; first done. *)
+ (*        rewrite /hist_to_we. *)
+ (*        assert (Some hv = head (hv :: Hhv)) as Hsomehv by done. *)
+ (*        rewrite -last_reverse in Hsomehv. *)
+ (*        rewrite Hsomehv. *)
+ (*        rewrite reverse_cons. *)
+ (*        rewrite last_snoc. *)
+ (*        assert ((reverse h) `suffix_of` ((hv :: Hhv))) as Hsuf. *)
+ (*        { rewrite Heq2 in Hpre. *)
+ (*          admit. } *)
+ (*        admit. *)
+ (*      } *)
+ (*      wp_pure _. *)
+ (*      (* iApply ("IH" with "[$HΦ]"). *) *)
+ (*   Admitted. *)
 
   Lemma read_handler_spec
         (k : string)
@@ -164,14 +274,14 @@ Section Proof_of_read_handler.
     k ∈ KVS_keys →
     reqd = inl (k, ts, h) →
     (∀ e : events.write_event, e ∈ h → we_time e < ts) →
-    server_lock_inv γGauth γT γlk lk kvs vnum -∗
-    Global_Inv clients γKnownClients γGauth γGsnap γT -∗
-    ownTimeSnap γT ts -∗
+    server_lock_inv γGauth γT γTss γlk lk kvs vnum -∗
+    Global_Inv clients γKnownClients γGauth γGsnap γT γTss -∗
+    ownTimeSnap γT γTss ts -∗
     ownMemSeen γGsnap k h -∗
     (∀ (repv : val) (repd : RepData),
        ⌜sum_valid_val (option_serialization KVS_serialization)
         (sum_serialization int_serialization bool_serialization) repv⌝ ∗
-         ReqPost clients γKnownClients γGauth γGsnap γT repv reqd repd -∗
+         ReqPost clients γKnownClients γGauth γGsnap γT γTss repv reqd repd -∗
            Φ repv) -∗
     WP let: "res" := InjL
                      (acquire lk ;;
@@ -184,8 +294,8 @@ Section Proof_of_read_handler.
     iIntros (?) "(-> & Hlock & Hlkres)".
     wp_pures.
     iDestruct "Hlkres"
-      as (kvsV T m M Hmap Hvalid Hforall)
-           "(HmemLoc & HtimeLoc & HkvsL & HvnumL)".
+      as (kvsV T Tss m M Hmap Hvalid Hforall)
+           "(HmemLoc & HtimeLoc & #Hstarts & HkvsL & HvnumL)".
     wp_load.
     admit.
     (* wp_apply (kvs_get_last_spec); try done. eauto. *)
